hoisting a couple of nested recursive functions

src/tls/CommonDH.fst
@@ -438,8 +438,7 @@ let pinverse_keyShareEntry x = ()
 
 // Choice: truncate when maximum length is exceeded
 (** Serializing function for a list of KeyShareEntry *)
-let keyShareEntriesBytes kes =
-  let rec keyShareEntriesBytes_aux (b:bytes{length b < 65536}) (kes:list keyShareEntry): Tot (b:bytes{length b < 65536}) (decreases kes) =
+private let rec keyShareEntriesBytes_aux (b:bytes{length b < 65536}) (kes:list keyShareEntry): Tot (b:bytes{length b < 65536}) (decreases kes) =
   match kes with
   | [] -> b
   | ke::kes ->
@@ -447,29 +446,33 @@ let keyShareEntriesBytes kes =
     if length b' < 65536 then
       keyShareEntriesBytes_aux b' kes
     else b
-  in
+
+let keyShareEntriesBytes kes =
   let b = keyShareEntriesBytes_aux empty_bytes kes in
   lemma_repr_bytes_values (length b);
   vlbytes 2 b
 
 (** Parsing function for a list KeyShareEntry *)
-let parseKeyShareEntries b =
-  let rec (aux: b:bytes -> list keyShareEntry -> Tot (result (list keyShareEntry)) (decreases (length b))) = fun b entries ->
-    if length b > 0 then
+private let rec parseKeyShareEntries_aux (b:bytes) (entries:list keyShareEntry)
+   : Tot (result (list keyShareEntry)) 
+         (decreases (length b))
+   = if length b > 0 then
       if length b >= 4 then
 	let ng, data = split b 2ul in
 	match vlsplit 2 data with
 	| Correct(kex, bytes) ->
 	  begin
 	  match parseKeyShareEntry (ng @| vlbytes 2 kex) with
-	  | Correct entry -> aux bytes (entries @ [entry])
+	  | Correct entry -> parseKeyShareEntries_aux bytes (entries @ [entry])
 	  | Error z -> Error z
 	  end
 	| Error z -> Error(AD_decode_error, perror __SOURCE_FILE__ __LINE__ "Failed to parse key share entry")
       else Error (AD_decode_error, perror __SOURCE_FILE__ __LINE__ "Too few bytes to parse key share entries")
-    else Correct entries in
+    else Correct entries
+  
+let parseKeyShareEntries b =
   match vlparse 2 b with
-  | Correct b -> aux b []
+  | Correct b -> parseKeyShareEntries_aux b []
   | Error z   -> Error(AD_decode_error, perror __SOURCE_FILE__ __LINE__ "Failed to parse key share entries")
 
 (** Serializing function for a ClientKeyShare *)
